wip trying to sketch structure of pipeline/event loop proof and connection

compiler/src/PipelineWithRename.v
@@ -122,57 +122,138 @@ Section Pipeline1.
   Definition available_registers: list Register :=
     Eval cbv in List.unfoldn Z.succ 29 3.
 
-  Definition ExprImp2Riscv(s: @Syntax.cmd (FlattenExpr.FlattenExpr.mk_Syntax_params _)):
-    list Instruction :=
-    let flat := ExprImp2FlatImp s in
-    match rename_stmt string Register funname string map.empty flat available_registers with
-    | Some flat' => FlatToRiscvDef.compile_stmt flat'
-    | None => nil
-    end.
+  Local Notation cmd := (@Syntax.cmd (FlattenExpr.FlattenExpr.mk_Syntax_params _)).
+  Local Notation env := (@Semantics.env (FlattenExpr.mk_Semantics_params _)).
 
-  Definition ExprImp2RenamedFlat(s: @Syntax.cmd (FlattenExpr.FlattenExpr.mk_Syntax_params _)):
-    FlatImp.stmt :=
+  Definition functions2Riscv(e: env)(funs: list funname): list Instruction * fun_pos_env :=
+    let e' := flatten_functions e funs in
+    let e'' := rename_functions string Register funname string available_registers e' funs in
+    FlatToRiscvDef.compile_functions e'' funs.
+
+  Definition ExprImp2RenamedFlat(s: cmd): FlatImp.stmt :=
     let flat := ExprImp2FlatImp s in
     match rename_stmt string Register funname string map.empty flat available_registers with
     | Some flat' => flat'
     | None => FlatImp.SSkip
     end.
 
-  Local Notation cmd := (@Syntax.cmd (FlattenExpr.FlattenExpr.mk_Syntax_params _)).
-  Local Notation env := (@Semantics.env (FlattenExpr.mk_Semantics_params _)).
+  Definition snippet2Riscv(e_pos: fun_pos_env)(mypos: Z)(s: cmd): list Instruction :=
+    let flat := ExprImp2RenamedFlat s in
+    FlatToRiscvDef.compile_snippet e_pos mypos flat.
 
+(*
+  Definition goodMachine(e: env)(mH: mem)(st: MetricRiscvMachine): Prop :=
+    exists t l mc g,
+      functions2Riscv e funs = (g.(insts)
+      FlatToRiscvFunctions.goodMachine t mH l mc g st.
+*)
+
+  Definition goodMachine: MetricRiscvMachine -> Prop. Admitted.
+
+  Lemma exprImp2Riscv_correct: forall (e: env) (sH: cmd) lH mH mcH t program_base e_pos pos
+                                      (initialL: MetricRiscvMachine) post instsL,
+      snippet2Riscv e_pos pos sH = instsL ->
+      Semantics.exec.exec e sH t mH lH mcH post ->
+      initialL.(getPc) = word.add program_base (word.of_Z pos) ->
+      goodMachine initialL ->
+      runsTo initialL (fun finalL => exists t' mH' lH' mcH',
+          post t' mH' lH' mcH' /\
+          finalL.(getPc) = word.add initialL.(getPc)
+                                   (word.of_Z (4 * Z.of_nat (List.length instsL))) /\
+          goodMachine finalL).
+  Admitted.
+
+(*
   Lemma exprImp2Riscv_correct: forall (e: env) (sH: cmd) lH mH mcH t instsL
-                                      (initialL: MetricRiscvMachine) post,
+                                      (initialL: MetricRiscvMachine) post R,
       @ExprImp.cmd_size (FlattenExpr.mk_Semantics_params _) sH < 2 ^ 10 ->
       ExprImp2Riscv sH = instsL ->
       (word.unsigned initialL.(getPc)) mod 4 = 0 ->
       initialL.(getNextPc) = word.add initialL.(getPc) (word.of_Z 4) ->
       initialL.(getLog) = t ->
-      (program initialL.(getPc) instsL * eq mH)%sep initialL.(getMem) ->
+      (program initialL.(getPc) instsL * eq mH * R)%sep initialL.(getMem) ->
       ext_guarantee initialL ->
       Semantics.exec.exec e sH t mH lH mcH post ->
       runsToNonDet.runsTo (mcomp_sat (run1 iset))
              initialL
              (fun finalL => exists mH' lH' mcH',
                   post finalL.(getLog) mH' lH' mcH' /\
-                  (*map.extends finalL.(getRegs) lH' /\*)
-                  (program initialL.(getPc) (ExprImp2Riscv sH) * eq mH')%sep (getMem finalL)).
-  Admitted.
-
-(*
-  Definition compile_functions(e: Semantics.env)(funnames: list funname): list Instruction :=
-    FlatToRiscvDef.compile_functions (flatten_functions e funnames) funnames.
+                  map.extends finalL.(getRegs) lH' /\
+                  (program initialL.(getPc) (ExprImp2Riscv sH) * eq mH' * R)%sep (getMem finalL) /\
+                  getPc finalL = add (getPc initialL) (mul (ZToReg 4) (ZToReg (Zlength instsL))) /\
+                  getNextPc finalL = add (getPc finalL) (ZToReg 4)).
+  Proof.
+    intros. subst.
+    eapply runsTo_weaken. Unshelve.
+    - eapply FlatToRiscvMetric.compile_stmt_correct
+          with (postH := (fun t m l mc =>
+                            exists l' mc',
+                              post t m l' mc' /\
+                              map.extends l l' /\
+                              (mc - mcH <= mc' - mcH)%metricsH)
+               ); try reflexivity.
+      + eapply FlatImp.exec.weaken.
+        * match goal with
+          | |- _ ?env ?s ?t ?m ?l ?mc ?post =>
+            epose proof (@FlattenExpr.flattenStmt_correct _ _ _ _ _ _ _ _ _ eq_refl) as Q
+          end.
+          eapply Q.
+          eassumption.
+        * simpl. intros. simp. do 2 eexists. do 2 (split; try eassumption).
+      + unfold FlatToRiscvDef.stmt_not_too_big.
+        unfold ExprImp2Riscv, ExprImp2FlatImp in *.
+        match goal with
+        | |- context [fst ?x] => destruct x eqn: E
+        end.
+        match goal with
+        | H: _ = (?a, ?b) |- context [fst ?x] => replace x with (a, b) by reflexivity
+        end.
+        unfold fst.
+        apply FlattenExpr.flattenStmt_size in E.
+        ineq_step.
+        destruct E as [_ E].
+        simpl in *.
+        (* TODO why do blia and blia fail here? PARAMRECORDS? *)
+        Fail blia. Fail blia.
+        exact E.
+      + unfold enough_registers, ExprImp2FlatImp, fst in *. assumption.
+      + assumption.
+      + match goal with
+        | H: context [ program _ ?insts ] |- context [ program _ ?insts' ] =>
+          change insts' with insts
+        end.
+        simpl in *.
+        seplog.
+      + assumption.
+      + assumption.
+    - simpl. intros. simp. do 3 eexists. do 3 (split; try eassumption).
+      split; [assumption|].
+      split; [assumption|].
+      solve_MetricLog.
+  Qed.
 *)
 
-  Definition compile_prog(e: env) (init_sp: Z) (init_code loop_body: cmd)
-             (funs: list funname): list Instruction :=
-    let e' := flatten_functions e funs in
-    let e'' := rename_functions string Register funname string available_registers e' funs in
+  (* uses relative jumps for function calls and expects that the compiled functions will be
+     put right after the code returned by this compilation function *)
+  Definition compile_main(e_pos: fun_pos_env)(init_code loop_body: cmd): list Instruction :=
     (* TODO the two below should share local variables and not rename independently *)
     let init_code' := ExprImp2RenamedFlat init_code in
     let loop_body' := ExprImp2RenamedFlat loop_body in
+    let main_size := List.length (FlatToRiscvDef.compile_main e_pos 42 init_code' loop_body') in
+    FlatToRiscvDef.compile_main e_pos (- 4 * Z.of_nat main_size) init_code' loop_body'.
+
+  Definition compile_prog(e: env)(init_sp: Z)(init_code loop_body: cmd)(funs: list funname):
+    list Instruction :=
+    (* all positions in e_pos are relative to the position of the first function *)
+    let '(fun_insts, e_pos) := functions2Riscv e funs in
     FlatToRiscvDef.compile_lit RegisterNames.sp init_sp ++
-    FlatToRiscvDef.compile_prog e'' init_code' loop_body' funs.
+    compile_main e_pos init_code loop_body ++
+    fun_insts.
+
+  Definition putProgram(e: env)(funs: list funname)(init_code loop_body: cmd)(code_addr: word)
+             (stack_pastend: word)(preInitial: MetricRiscvMachine): MetricRiscvMachine :=
+    let insts := compile_prog e (word.unsigned stack_pastend) init_code loop_body funs in
+    MetricRiscvMachine.putProgram (List.map encode insts) code_addr preInitial.
 
   Add Ring wring : (word.ring_theory (word := word))
       (preprocess [autorewrite with rew_word_morphism],
@@ -195,6 +276,7 @@ Section Pipeline1.
                                    Semantics.exec e loop_body t m l mc hl_ready)
       (code_area_begin: word)
       (code_area_begin_aligned: word.unsigned code_area_begin mod 4 = 0)
+      (stack_area_begin stack_area_pastend: word)
       (insts_init: list Instruction)
       (insts_body: list Instruction)
       (* technical detail: "pc at beginning of loop" and "pc at end of loop" needs to be
@@ -208,6 +290,12 @@ Section Pipeline1.
     word.add code_area_begin (word.of_Z (4 * Z.of_nat (List.length insts_init))).
 
   Definition ll_ready(st: MetricRiscvMachine): Prop :=
+    exists regsH memH metricsH,
+      hl_ready st.(getLog) memH regsH metricsH /\
+      goodMachine st.
+
+(*
+  Definition ll_ready(st: MetricRiscvMachine): Prop :=
       exists regsH memH metricsH R p_stacklimit p_sp stack_trash initial_pc program_base
       e_pos e_impl,
         hl_ready st.(getLog) memH regsH metricsH /\
@@ -215,8 +303,16 @@ Section Pipeline1.
         (R * eq memH * @word_array FlatToRisvc_params p_stacklimit stack_trash *
          program initial_pc insts_init * program pc_start insts_body *
          @functions FlatToRisvc_params program_base e_pos e_impl funnames)%sep st.(getMem).
+*)
 
   Definition ll_inv: MetricRiscvMachine -> Prop := runsToGood_Invariant ll_ready pc_start.
+
+  Lemma putProgram_establishes_ll_inv: forall preInitial initial,
+      initial = (putProgram e funnames init_code loop_body code_area_begin stack_area_pastend
+                            preInitial) ->
+      ll_inv initial.
+  Proof.
+  Admitted.
 
   Lemma ll_inv_is_invariant: forall st: MetricRiscvMachine,
       ll_inv st -> mcomp_sat (run1 iset) st ll_inv.
@@ -231,6 +327,10 @@ Section Pipeline1.
              | |- _ /\ _ => split
              | |- _ => eassumption
              end.
+      match goal with
+      | A: ?G |- ?G' => replace G' with G; [exact A|progress f_equal]
+      end.
+      f_equal. 2: admit. f_equal. all: admit.
     - unfold pc_start. solve_divisibleBy4.
     - admit.
     - admit.
@@ -238,19 +338,21 @@ Section Pipeline1.
     - solve_word_eq word_ok.
     - (* use compiler correctness for init_code *)
       eapply runsTo_weaken.
-      + eapply exprImp2Riscv_correct; cycle -1.
-        1: exact exec_init.
-        all: try reflexivity; admit.
-      + simpl. intros. unfold ll_ready.
+      + eapply exprImp2Riscv_correct; try exact exec_init; try reflexivity.
+        (* establish goodMachine & other sideconditions of exprImp2Riscv_correct *)
+        all: admit.
+      + simpl. intros. unfold ll_ready. simp.
+        repeat eexists. 1: { Fail exact H0. admit. }
         (* TODO: guarantee from exprImp2Riscv_correct needs to be stronger *)
-        admit.
+        all: admit.
     - (* use compiler correctness for loop_body *)
       intros.
       eapply runsTo_weaken.
       + unfold ll_ready in *. simp.
-        eapply exprImp2Riscv_correct; cycle -1.
+        eapply exprImp2Riscv_correct.
+        1: reflexivity.
         1: { eapply exec_body. eassumption. }
-        all: try reflexivity; admit.
+        all: admit.
       + simpl. intros. unfold ll_ready.
         (* TODO: guarantee from exprImp2Riscv_correct needs to be stronger *)
         admit.
@@ -267,17 +369,18 @@ Section Pipeline1.
     eapply hl_ready_implies_hl_inv. eassumption.
   Qed.
 
-  Lemma compile_prog_correct:
-      (* there exists a low-level invariant which is somewhat complex and therefore not exposed *)
-      exists ll_inv: MetricRiscvMachine -> Prop,
-        (* how a client can establish ll_inv: *)
-        (forall st: MetricRiscvMachine,
-            True ->
-            ll_inv st) /\
-        (* how a client can use ll_inv: *)
-        (forall st: MetricRiscvMachine, ll_inv st -> mcomp_sat (run1 iset) st ll_inv /\
-                                                     exists suff, hl_inv (suff ++ st.(getLog))).
+  Lemma pipeline_proofs:
+    (forall preInitial initial,
+        initial = (putProgram e funnames init_code loop_body code_area_begin stack_area_pastend
+                              preInitial) ->
+        ll_inv initial) /\
+    (forall st, ll_inv st -> mcomp_sat (run1 iset) st ll_inv) /\
+    (forall st, ll_inv st -> exists suff, hl_inv (suff ++ st.(getLog))).
   Proof.
-  Admitted.
+    split; [|split].
+    - exact putProgram_establishes_ll_inv.
+    - exact ll_inv_is_invariant.
+    - exact ll_inv_implies_prefix_of_good.
+  Qed.
 
 End Pipeline1.
