compiler/src/Pipeline.v
@@ -113,9 +113,6 @@ Section Pipeline1.
   Definition ExprImp2Riscv(s: Syntax.cmd): list Instruction :=
     FlatToRiscvDef.compile_stmt (ExprImp2FlatImp s).
 
-  Definition compile_functions(e: Semantics.env)(funnames: list funname): list Instruction :=
-    FlatToRiscvDef.compile_functions (flatten_functions e funnames) funnames.
-
   Definition compile_prog(e: Semantics.env)(s: Syntax.cmd)(funs: list funname): list Instruction :=
     let e' := flatten_functions e funs in
     let s' := ExprImp2FlatImp s in
